shift-reset/interpreter/interpreter.v
@@ -1,132 +1,21 @@
-From Stdlib Require Import String ZArith Lia.
-From shift_reset.core Require Import syntax var env.
-From shift_reset.interpreter Require Import istate ierror imonad.
+From Stdlib Require Import String ZArith.
+From shift_reset.core Require Import syntax env loc var.
+From shift_reset.interpreter Require Import ierror iheap imonad.
 
 Local Open Scope string_scope.
+Local Open Scope Z_scope.
 
 Definition interpret_atom (a : atom) : imonad val :=
   match a with
   | AUnit => imonad_pure VUnit
   | AInt i => imonad_pure (VInt i)
   | ABool b => imonad_pure (VBool b)
-  | AVar x =>
-      imonad_bind imonad_ask_env
-        (fun env => match env_lookup x env with
-                    | None => imonad_throw (NameError (var_car x))
-                    | Some v => imonad_pure v
-                    end)
+  | AVar x => imonad_bind imonad_ask_env
+                (fun env => match env_lookup x env with
+                            | None => imonad_throw (NameError (var_car x))
+                            | Some v => imonad_pure v
+                            end)
   end.
-
-Definition interpret_term1_aux (go : term -> imonad val) (t : term1) (v : val) : imonad val :=
-  let (b, t') := t in
-  let m := go t' in
-  match b with
-  | BAnon => m
-  | BVar x => imonad_local_env (ECons x v) m
-  end.
-
-Definition interpret_term2_aux (go : term -> imonad val) (t : term2) (v1 v2 : val) : imonad val :=
-  let (b, t') := t in
-  match b with
-  | BAnon => interpret_term1_aux go t' v2
-  | BVar x => imonad_local_env (ECons x v1) (interpret_term1_aux go t' v2)
-  end.
-
-Definition interpret_clo1_aux (go : term -> imonad val) (c : clo1) (v : val) : imonad val :=
-  let (env, t) := c in imonad_local_env (fun _ => env) (interpret_term1_aux go t v).
-
-Definition interpret_clo2_aux (go : term -> imonad val) (c : clo2) (v1 v2 : val) : imonad val :=
-  let (env, t) := c in imonad_local_env (fun _ => env) (interpret_term2_aux go t v1 v2).
-
-Definition interpret_if (a : atom) (m1 m2 : imonad val) :=
-  imonad_bind (interpret_atom a)
-    (fun v => match v with
-              | VBool b => if b then m1 else m2
-              | _ => imonad_throw (TypeError "")
-              end).
-
-Local Open Scope Z_scope.
-
-Definition interpret_prim1 (p : prim1) (a : atom) : imonad val :=
-  imonad_bind (interpret_atom a)
-    (fun v => match p, v with
-              | P1Neg, VInt i => imonad_pure (VInt (-i))
-              | P1Not, VBool b => imonad_pure (VBool (negb b))
-              | _, _ => imonad_throw (TypeError "")
-              end).
-
-Definition interpret_prim2 (p : prim2) (a1 a2 : atom) : imonad val :=
-  let m1 := interpret_atom a1 in
-  let m2 := interpret_atom a2 in
-  imonad_bind m1
-    (fun v1 =>
-       match p, v1 with
-       | P2Add, VInt i1 =>
-           imonad_bind m2
-             (fun v2 => match v2 with
-                        | VInt i2 => imonad_pure (VInt (i1 + i2))
-                        | _ => imonad_throw (TypeError "")
-                        end)
-       | P2Sub, VInt i1 =>
-           imonad_bind m2
-             (fun v2 => match v2 with
-                        | VInt i2 => imonad_pure (VInt (i1 - i2))
-                        | _ => imonad_throw (TypeError "")
-                        end)
-       | P2Mul, VInt i1 =>
-           imonad_bind m2
-             (fun v2 => match v2 with
-                        | VInt i2 => imonad_pure (VInt (i1 * i2))
-                        | _ => imonad_throw (TypeError "")
-                        end)
-       | P2Div, VInt i1 =>
-           imonad_bind m2
-             (fun v2 => match v2 with
-                        | VInt i2 => imonad_pure (VInt (i1 / i2))
-                        | _ => imonad_throw (TypeError "")
-                        end)
-       | P2Rem, VInt i1 =>
-           imonad_bind m2
-             (fun v2 => match v2 with
-                        | VInt i2 => imonad_pure (VInt (Z.rem i1 i2))
-                        | _ => imonad_throw (TypeError "")
-                        end)
-       | P2Lt, VInt i1 =>
-           imonad_bind m2
-             (fun v2 => match v2 with
-                        | VInt i2 => imonad_pure (VBool (i1 <? i2))
-                        | _ => imonad_throw (TypeError "")
-                        end)
-       | P2Le, VInt i1 =>
-           imonad_bind m2
-             (fun v2 => match v2 with
-                        | VInt i2 => imonad_pure (VBool (i1 <=? i2))
-                        | _ => imonad_throw (TypeError "")
-                        end)
-       | P2And, VBool b1 =>
-           imonad_bind m2
-             (fun v2 => match v2 with
-                        | VBool b2 => imonad_pure (VBool (b1 && b2))
-                        | _ => imonad_throw (TypeError "")
-                        end)
-       | P2Or, VBool b1 =>
-           imonad_bind m2
-             (fun v2 => match v2 with
-                        | VBool b2 => imonad_pure (VBool (b1 || b2))
-                        | _ => imonad_throw (TypeError "")
-                        end)
-       | P2Xor, VBool b1 =>
-           imonad_bind m2
-             (fun v2 => match v2 with
-                        | VBool b2 => imonad_pure (VBool (xorb b1 b2))
-                        | _ => imonad_throw (TypeError "")
-                        end)
-       | P2Eq, _ => imonad_bind m2 (fun v2 => imonad_pure (VBool (val_eqb v1 v2)))
-       | P2Neq, _ => imonad_bind m2 (fun v2 => imonad_pure (VBool (val_neqb v1 v2)))
-       | _, _ => imonad_throw (TypeError "")
-       end).
-
-Local Close Scope Z_scope.
 
 Definition interpret_fun (t : term1) : imonad val :=
   imonad_map (fun env => VFun (C1 env t)) imonad_ask_env.
@@ -134,20 +23,77 @@ Definition interpret_fun (t : term1) : imonad val :=
 Definition interpret_fix (t : term2) : imonad val :=
   imonad_map (fun env => VFix (C2 env t)) imonad_ask_env.
 
-Definition interpret_pair (a1 a2 : atom) : imonad val :=
-  imonad_lift2 VPair (interpret_atom a1) (interpret_atom a2).
-
-Definition interpret_fst (a : atom) : imonad val :=
-  imonad_bind (interpret_atom a)
+Definition unwrap_VInt_then (m : imonad val) (k : Z -> imonad val) : imonad val :=
+  imonad_bind m
     (fun v => match v with
-              | VPair v1 _ => imonad_pure v1
+              | VInt i => k i
               | _ => imonad_throw (TypeError "")
               end).
 
-Definition interpret_snd (a : atom) : imonad val :=
+Definition unwrap_VBool_then (m : imonad val) (k : bool -> imonad val) : imonad val :=
+  imonad_bind m
+    (fun v => match v with
+              | VBool b => k b
+              | _ => imonad_throw (TypeError "")
+              end).
+
+Definition unwrap_VLoc_then (m : imonad val) (k : loc -> imonad val) : imonad val :=
+  imonad_bind m
+    (fun v => match v with
+              | VLoc l => k l
+              | _ => imonad_throw (TypeError "")
+              end).
+
+Definition interpret_if (a : atom) (m1 m2 : imonad val) : imonad val :=
+  unwrap_VBool_then (interpret_atom a) (fun b => if b then m1 else m2).
+
+Definition interpret_i2i (f : Z -> Z) (m : imonad val) : imonad val :=
+  unwrap_VInt_then m (fun i => imonad_pure (VInt (f i))).
+
+Definition interpret_b2b (f : bool -> bool) (m : imonad val) : imonad val :=
+  unwrap_VBool_then m (fun b => imonad_pure (VBool (f b))).
+
+Definition interpret_prim1 (p : prim1) (a : atom) : imonad val :=
+  let m := interpret_atom a in
+  match p with
+  | P1Neg => interpret_i2i Z.opp m
+  | P1Not => interpret_b2b negb m
+  end.
+
+Definition interpret_ii2i (f : Z -> Z -> Z) (m1 m2 : imonad val) : imonad val :=
+  unwrap_VInt_then m1 (fun i1 => unwrap_VInt_then m2 (fun i2 => imonad_pure (VInt (f i1 i2)))).
+
+Definition interpret_ii2b (f : Z -> Z -> bool) (m1 m2 : imonad val) : imonad val :=
+  unwrap_VInt_then m1 (fun i1 => unwrap_VInt_then m2 (fun i2 => imonad_pure (VBool (f i1 i2)))).
+
+Definition interpret_bb2b (f : bool -> bool -> bool) (m1 m2 : imonad val) : imonad val :=
+  unwrap_VBool_then m1 (fun b1 => unwrap_VBool_then m2 (fun b2 => imonad_pure (VBool (f b1 b2)))).
+
+Definition interpret_prim2 (p : prim2) (a1 a2 : atom) : imonad val :=
+  let m1 := interpret_atom a1 in
+  let m2 := interpret_atom a2 in
+  match p with
+  | P2Add => interpret_ii2i Z.add m1 m2
+  | P2Sub => interpret_ii2i Z.sub m1 m2
+  | P2Mul => interpret_ii2i Z.mul m1 m2
+  | P2Div => interpret_ii2i Z.div m1 m2
+  | P2Rem => interpret_ii2i Z.rem m1 m2
+  | P2Lt => interpret_ii2b Z.ltb m1 m2
+  | P2Le => interpret_ii2b Z.leb m1 m2
+  | P2And => interpret_bb2b andb m1 m2
+  | P2Or => interpret_bb2b orb m1 m2
+  | P2Xor => interpret_bb2b xorb m1 m2
+  | P2Eq => imonad_lift2 (fun v1 v2 => VBool (val_eqb v1 v2)) m1 m2
+  | P2Neq => imonad_lift2 (fun v1 v2 => VBool (val_neqb v1 v2)) m1 m2
+  end.
+
+Definition interpret_pair (a1 a2 : atom) : imonad val :=
+  imonad_lift2 VPair (interpret_atom a1) (interpret_atom a2).
+
+Definition interpret_split (a : atom) (k : val -> val -> imonad val) : imonad val :=
   imonad_bind (interpret_atom a)
     (fun v => match v with
-              | VPair _ v2 => imonad_pure v2
+              | VPair v1 v2 => k v1 v2
               | _ => imonad_throw (TypeError "")
               end).
 
@@ -157,327 +103,341 @@ Definition interpret_inl (a : atom) : imonad val :=
 Definition interpret_inr (a : atom) : imonad val :=
   imonad_map VInr (interpret_atom a).
 
-Definition interpret_case (a : atom) (t1 t2 : val -> imonad val) : imonad val :=
+Definition interpret_case (a : atom) (k1 k2 : val -> imonad val) : imonad val :=
   imonad_bind (interpret_atom a)
     (fun v => match v with
-              | VInl v' => t1 v'
-              | VInr v' => t2 v'
+              | VInl v' => k1 v'
+              | VInr v' => k2 v'
               | _ => imonad_throw (TypeError "")
               end).
 
 Definition interpret_ref (a : atom) : imonad val :=
   imonad_bind (interpret_atom a)
-    (fun v =>
-       imonad_bind imonad_get_state
-         (fun s =>
-            match istate_ref v s with
-            | None => imonad_throw (MemoryError "")
-            | Some (l, s') => imonad_then (imonad_set_state s') (imonad_pure (VLoc l))
-            end)).
+    (fun v => imonad_bind imonad_get_heap
+                (fun h => match iheap_ref v h with
+                          | None => imonad_throw (MemoryError "")
+                          | Some (l, h') => imonad_then (imonad_set_heap h') (imonad_pure (VLoc l))
+                          end)).
 
 Definition interpret_get (a : atom) : imonad val :=
-  imonad_bind (interpret_atom a)
-    (fun v =>
-       match v with
-       | VLoc l =>
-           imonad_bind imonad_get_state
-             (fun s =>
-                match istate_get l s with
-                | None => imonad_throw (MemoryError "")
-                | Some v => imonad_pure v
-                end)
-       | _ => imonad_throw (TypeError "")
-       end).
+  unwrap_VLoc_then (interpret_atom a)
+    (fun l => imonad_bind imonad_get_heap
+                (fun h => match iheap_get l h with
+                          | None => imonad_throw (MemoryError "")
+                          | Some v => imonad_pure v
+                          end)).
 
 Definition interpret_set (a1 a2 : atom) : imonad val :=
   let m1 := interpret_atom a1 in
   let m2 := interpret_atom a2 in
-  imonad_bind m1
-    (fun v1 =>
-       match v1 with
-       | VLoc l =>
-           imonad_bind m2
-             (fun v2 =>
-                imonad_bind imonad_get_state
-                  (fun s =>
-                     match istate_set l v2 s with
-                     | None => imonad_throw (MemoryError "")
-                     | Some s' => imonad_then (imonad_set_state s') (imonad_pure VUnit)
-                     end))
-       | _ => imonad_throw (TypeError "")
-       end).
+  unwrap_VLoc_then m1
+    (fun l => imonad_bind m2
+                (fun v => imonad_bind imonad_get_heap
+                            (fun h => match iheap_set l v h with
+                                      | None => imonad_throw (MemoryError "")
+                                      | Some h' => imonad_then (imonad_set_heap h') (imonad_pure VUnit)
+                                      end))).
 
 Definition interpret_free (a : atom) : imonad val :=
-  imonad_bind (interpret_atom a)
-    (fun v =>
-       match v with
-       | VLoc l =>
-           imonad_bind imonad_get_state
-             (fun s =>
-                match istate_free l s with
-                | None => imonad_throw (MemoryError "")
-                | Some s' => imonad_then (imonad_set_state s') (imonad_pure VUnit)
-                end)
-       | _ => imonad_throw (TypeError "")
-       end).
+  unwrap_VLoc_then (interpret_atom a)
+    (fun l => imonad_bind imonad_get_heap
+                (fun h => match iheap_free l h with
+                          | None => imonad_throw (MemoryError "")
+                          | Some h' => imonad_then (imonad_set_heap h') (imonad_pure VUnit)
+                          end)).
 
-(*
-Section interpret_kont.
-  Context (go : forall (t : term) (k : kont), Acc lt (term_size t + kont_size k) -> imonad val).
-
-  Definition interpret_term1_kont_aux (t : term1) (k : kont) (H_acc : Acc lt (term1_size t + kont_size k)) (v : val) : imonad val :=
-    match t return Acc lt (term1_size t + kont_size k) -> imonad val with
-    | T1 b t' => fun H_acc =>
-                   let m := go t' k H_acc in
-                   match b with
-                   | BAnon => m
-                   | BVar x => imonad_local_env (ECons x v) m
-                   end
-    end H_acc.
-
-  Definition interpret_clo1_kont_aux (c : clo1) (k : kont) (H_acc : Acc lt (clo1_size c + kont_size k)) (v : val) : imonad val :=
-    match c return Acc lt (clo1_size c + kont_size k) -> imonad val with
-    | C1 env t => fun H_acc => imonad_local_env (fun _ => env) (interpret_term1_kont_aux t k H_acc v)
-    end H_acc.
-
-  Definition interpret_kont_aux (k : kont) (H_acc : Acc lt (kont_size k)) (m : imonad val) : imonad val :=
-    match k return Acc lt (kont_size k) -> imonad val with
-    | KNil => fun _ => m
-    | KCons c k' => fun H_acc => imonad_bind m (interpret_clo1_kont_aux c k' H_acc)
-    end H_acc.
-End interpret_kont.
-*)
-
-Definition interpret_kont (go : term -> kont -> imonad val) (k : kont) (m : imonad val) : imonad val :=
-  match k with
-  | KNil => m
-  | KCons c k' => imonad_bind m (interpret_clo1_aux (fun t => go t k') c)
-  end.
-
-Definition interpret_term1_aux'
-  (go : term -> kont -> (imonad val -> imonad val) -> imonad val)
-  (t : term1)
-  (k : kont)
-  (k_meta : imonad val -> imonad val)
-  (env : env)
-  (m : imonad val) :=
-  imonad_bind m (fun v =>
-                   let (b, t') := t in
-                   let m := go t' k k_meta in
-                   match b with
-                   | BAnon => imonad_local_env (fun _ => env) m
-                   | BVar x => imonad_local_env (fun _ => ECons x v env) m
-                   end).
-
-Definition interpret_term1_kont_aux
-  (go : term -> kont -> (imonad val -> imonad val) -> imonad val)
-  (t : term1)
-  (k : kont)
-  (k_meta : imonad val -> imonad val)
-  (v : val) :=
-  let (b, t') := t in
-  let m := go t' k k_meta in
+Definition with_binder (b : binder) (v : val) (m : imonad val) : imonad val :=
   match b with
   | BAnon => m
   | BVar x => imonad_local_env (ECons x v) m
   end.
 
-Definition interpret_clo1_kont_aux
-  (go : term -> kont -> (imonad val -> imonad val) -> imonad val)
-  (c : clo1)
-  (k : kont)
-  (k_meta : imonad val -> imonad val)
-  (v : val) :=
-  let (env, t) := c in
-  imonad_local_env (fun _ => env) (interpret_term1_kont_aux go t k k_meta v).
+Definition with_env (env : env) : imonad val -> imonad val :=
+  imonad_local_env (fun _ => env).
 
-Definition interpret_term_kont_aux (go : term -> kont -> (imonad val -> imonad val) -> imonad val) :
-  term -> kont -> (imonad val -> imonad val) -> imonad val :=
-  fix go' t k k_meta {struct t} :=
-    match t with
-    | TAtom a => k_meta (interpret_atom a)
-    | TLet t1 t2 =>
-        imonad_bind imonad_ask_env
-          (fun env =>
-             let c := C1 env t2 in
-             go' t1 (KCons c k) (fun m => imonad_bind m (interpret_clo1_kont_aux go' c k k_meta)))
-    | TIf a t1 t2 => interpret_if a (go' t1 k k_meta) (go' t2 k k_meta)
-    | TPrim1 p a => k_meta (interpret_prim1 p a)
-    | TPrim2 p a1 a2 => k_meta (interpret_prim2 p a1 a2)
-    | TFun t' => k_meta (interpret_fun t')
-    | TFix t' => k_meta (interpret_fix t')
-    (*| TApp a1 a2 => fun H_acc =>
-                      let m1 := interpret_atom a1 in
-                      let m2 := interpret_atom a2 in
-                      imonad_bind m1
-                        (fun v1 =>
-                           match v1 with
-                           | VFun c => imonad_bind m2 (interpret_clo1_aux (fun t' => go t' k) c)
-                           | VFix c => imonad_bind m2 (interpret_clo2_aux (fun t' => go t' k) c v1)
-                           | VKont k' => interpret_kont_aux go' k _ (interpret_kont go k'  m2)
-                           | _ => imonad_throw (TypeError "")
-                           end)*)
-    | TPair a1 a2 => k_meta (interpret_pair a1 a2)
-    | TFst a => k_meta (interpret_fst a)
-    | TSnd a => k_meta (interpret_snd a)
-    | TInl a => k_meta (interpret_inl a)
-    | TInr a => k_meta (interpret_inr a)
-    (*| TCase a t1 t2 => fun H_acc => interpret_case a (interpret_term1_kont_aux go' t1 k _) (interpret_term1_kont_aux go' t2 k _)*)
-    | TRef a => k_meta (interpret_ref a)
-    | TGet a => k_meta (interpret_get a)
-    | TSet a1 a2 => k_meta (interpret_set a1 a2)
-    | TFree a => k_meta (interpret_free a)
-    | TShift t' => (*fun H_acc => interpret_term1_kont_aux go' t' KNil _ (VKont k)*)
-        interpret_term1_kont_aux go' t' KNil (fun m => m) (VKont k)
-    | TReset t' => k_meta (go' t' KNil (fun m => m))
-    | _ => imonad_throw (ControlError "todo")
-    end.
+Definition interpret_term1_with (rec : term -> imonad val) (t : term1) (m : imonad val) : imonad val :=
+  imonad_bind m (fun v => let (b, t') := t in with_binder b v (rec t')).
 
-Fixpoint interpret_term_kont (fuel : nat) (t : term) (k : kont) (k_meta : imonad val -> imonad val) : imonad val :=
-  match fuel with
-  | O => imonad_throw OutOfFuel
-  | S fuel' => interpret_term_kont_aux (interpret_term_kont fuel') t k k_meta
+Definition interpret_term2_with (rec : term -> imonad val) (t : term2) (v : val) (m : imonad val) : imonad val :=
+  imonad_bind m (fun v' => let (b1, b2, t') := t in with_binder b1 v (with_binder b2 v' (rec t'))).
+
+Definition interpret_clo1_with (rec : term -> imonad val) (c : clo1) (m : imonad val) : imonad val :=
+  let (env, t) := c in with_env env (interpret_term1_with rec t m).
+
+Definition interpret_clo2_with (rec : term -> imonad val) (c : clo2) (v : val) (m : imonad val) : imonad val :=
+  let (env, t) := c in with_env env (interpret_term2_with rec t v m).
+
+Definition interpret_kont_with (rec : term -> kont -> imonad val) (k : kont) (m : imonad val) : imonad val :=
+  match k with
+  | KNil => m
+  | KCons c k' => interpret_clo1_with (fun t => rec t k') c m
   end.
 
-Definition interpret_term_aux (go : term -> imonad val) (go_kont : term -> kont -> (imonad val -> imonad val) -> imonad val) : term -> imonad val :=
-  fix go' t {struct t} :=
-    match t with
-    | TAtom a => interpret_atom a
-    | TLet t1 t2 => imonad_bind (go' t1) (interpret_term1_aux go' t2)
-    | TIf a t1 t2 => interpret_if a (go' t1) (go' t2)
-    | TPrim1 p a => interpret_prim1 p a
-    | TPrim2 p a1 a2 => interpret_prim2 p a1 a2
-    | TFun t' => interpret_fun t'
-    | TFix t' => interpret_fix t'
-    | TApp a1 a2 => let m1 := interpret_atom a1 in
+Set Implicit Arguments.
+
+Inductive term_kont_graph : term -> kont -> Prop :=
+| GTAtom a k : kont_graph k -> term_kont_graph (TAtom a) k
+| GTFun t k : kont_graph k -> term_kont_graph (TFun t) k
+| GTFix t k : kont_graph k -> term_kont_graph (TFix t) k
+| GTApp a1 a2 k : kont_graph k -> term_kont_graph (TApp a1 a2) k
+| GTLet t1 t2 k : (forall env, term_kont_graph t1 (KCons (C1 env t2) k)) -> term_kont_graph (TLet t1 t2) k
+| GTIf a t1 t2 k : term_kont_graph t1 k -> term_kont_graph t2 k -> term_kont_graph (TIf a t1 t2) k
+| GTPrim1 p a k : kont_graph k -> term_kont_graph (TPrim1 p a) k
+| GTPrim2 p a1 a2 k : kont_graph k -> term_kont_graph (TPrim2 p a1 a2) k
+| GTPair a1 a2 k : kont_graph k -> term_kont_graph (TPair a1 a2) k
+| GTSplit a t k : term2_kont_graph t k -> term_kont_graph (TSplit a t) k
+| GTInl a k : kont_graph k -> term_kont_graph (TInl a) k
+| GTInr a k : kont_graph k -> term_kont_graph (TInr a) k
+| GTCase a t1 t2 k : term1_kont_graph t1 k -> term1_kont_graph t2 k -> term_kont_graph (TCase a t1 t2) k
+| GTRef a k : kont_graph k -> term_kont_graph (TRef a) k
+| GTGet a k : kont_graph k -> term_kont_graph (TGet a) k
+| GTSet a1 a2 k : kont_graph k -> term_kont_graph (TSet a1 a2) k
+| GTFree a k : kont_graph k -> term_kont_graph (TFree a) k
+| GTShift t k : term1_kont_graph t KNil -> term_kont_graph (TShift t) k
+| GTReset t k : term_kont_graph t KNil -> kont_graph k -> term_kont_graph (TReset t) k
+with term1_kont_graph : term1 -> kont -> Prop :=
+| GT1 b t k : term_kont_graph t k -> term1_kont_graph (T1 b t) k
+with term2_kont_graph : term2 -> kont -> Prop :=
+| GT2 b1 b2 t k : term_kont_graph t k -> term2_kont_graph (T2 b1 b2 t) k
+with clo1_kont_graph : clo1 -> kont -> Prop :=
+| GC1 env t k : term1_kont_graph t k -> clo1_kont_graph (C1 env t) k
+with kont_graph : kont -> Prop :=
+| GKNil : kont_graph KNil
+| GKCons c k : clo1_kont_graph c k -> kont_graph (KCons c k).
+
+Lemma GTAtom_inv : forall a k, term_kont_graph (TAtom a) k -> kont_graph k.
+Proof. inversion 1; auto. Defined.
+
+Lemma GTFun_inv : forall t k, term_kont_graph (TFun t) k -> kont_graph k.
+Proof. inversion 1; auto. Defined.
+
+Lemma GTFix_inv : forall t k, term_kont_graph (TFix t) k -> kont_graph k.
+Proof. inversion 1; auto. Defined.
+
+Lemma GTApp_inv : forall a1 a2 k, term_kont_graph (TApp a1 a2) k -> kont_graph k.
+Proof. inversion 1; auto. Defined.
+
+Lemma GTLet_inv : forall t1 t2 k, term_kont_graph (TLet t1 t2) k -> forall env, term_kont_graph t1 (KCons (C1 env t2) k).
+Proof. inversion 1; auto. Defined.
+
+Lemma GTIf_inv1 : forall a t1 t2 k, term_kont_graph (TIf a t1 t2) k -> term_kont_graph t1 k.
+Proof. inversion 1; auto. Defined.
+
+Lemma GTIf_inv2 : forall a t1 t2 k, term_kont_graph (TIf a t1 t2) k -> term_kont_graph t2 k.
+Proof. inversion 1; auto. Defined.
+
+Lemma GTPrim1_inv : forall p a k, term_kont_graph (TPrim1 p a) k -> kont_graph k.
+Proof. inversion 1; auto. Defined.
+
+Lemma GTPrim2_inv : forall p a1 a2 k, term_kont_graph (TPrim2 p a1 a2) k -> kont_graph k.
+Proof. inversion 1; auto. Defined.
+
+Lemma GTPair_inv : forall a1 a2 k, term_kont_graph (TPair a1 a2) k -> kont_graph k.
+Proof. inversion 1; auto. Defined.
+
+Lemma GTSplit_inv : forall a t k, term_kont_graph (TSplit a t) k -> term2_kont_graph t k.
+Proof. inversion 1; auto. Defined.
+
+Lemma GTInl_inv : forall a k, term_kont_graph (TInl a) k -> kont_graph k.
+Proof. inversion 1; auto. Defined.
+
+Lemma GTInr_inv : forall a k, term_kont_graph (TInr a) k -> kont_graph k.
+Proof. inversion 1; auto. Defined.
+
+Lemma GTCase_inv1 : forall a t1 t2 k, term_kont_graph (TCase a t1 t2) k -> term1_kont_graph t1 k.
+Proof. inversion 1; auto. Defined.
+
+Lemma GTCase_inv2 : forall a t1 t2 k, term_kont_graph (TCase a t1 t2) k -> term1_kont_graph t2 k.
+Proof. inversion 1; auto. Defined.
+
+Lemma GTRef_inv : forall a k, term_kont_graph (TRef a) k -> kont_graph k.
+Proof. inversion 1; auto. Defined.
+
+Lemma GTGet_inv : forall a k, term_kont_graph (TGet a) k -> kont_graph k.
+Proof. inversion 1; auto. Defined.
+
+Lemma GTSet_inv : forall a1 a2 k, term_kont_graph (TSet a1 a2) k -> kont_graph k.
+Proof. inversion 1; auto. Defined.
+
+Lemma GTFree_inv : forall a k, term_kont_graph (TFree a) k -> kont_graph k.
+Proof. inversion 1; auto. Defined.
+
+Lemma GTShift_inv : forall t k, term_kont_graph (TShift t) k -> term1_kont_graph t KNil.
+Proof. inversion 1; auto. Defined.
+
+Lemma GTReset_inv1 : forall t k, term_kont_graph (TReset t) k -> term_kont_graph t KNil.
+Proof. inversion 1; auto. Defined.
+
+Lemma GTReset_inv2 : forall t k, term_kont_graph (TReset t) k -> kont_graph k.
+Proof. inversion 1; auto. Defined.
+
+Lemma GT1_inv : forall b t k, term1_kont_graph (T1 b t) k -> term_kont_graph t k.
+Proof. inversion 1; auto. Defined.
+
+Lemma GT2_inv : forall b1 b2 t k, term2_kont_graph (T2 b1 b2 t) k -> term_kont_graph t k.
+Proof. inversion 1; auto. Defined.
+
+Lemma GC1_inv : forall env t k, clo1_kont_graph (C1 env t) k -> term1_kont_graph t k.
+Proof. inversion 1; auto. Defined.
+
+Lemma GKCons_inv : forall c k, kont_graph (KCons c k) -> clo1_kont_graph c k.
+Proof. inversion 1; auto. Defined.
+
+Fixpoint compute_term_kont_graph_dep (t : term) (k : kont) (G : kont_graph k) : term_kont_graph t k :=
+  match t with
+  | TAtom a => GTAtom a G
+  | TFun t' => GTFun t' G
+  | TFix t' => GTFix t' G
+  | TApp a1 a2 => GTApp a1 a2 G
+  | TLet t1 t2 => GTLet (fun env => compute_term_kont_graph_dep t1 (GKCons (GC1 env (compute_term1_kont_graph_dep t2 G))))
+  | TIf a t1 t2 => GTIf a (compute_term_kont_graph_dep t1 G) (compute_term_kont_graph_dep t2 G)
+  | TPrim1 p a => GTPrim1 p a G
+  | TPrim2 p a1 a2 => GTPrim2 p a1 a2 G
+  | TPair a1 a2 => GTPair a1 a2 G
+  | TSplit a t' => GTSplit a (compute_term2_kont_graph_dep t' G)
+  | TInl a => GTInl a G
+  | TInr a => GTInr a G
+  | TCase a t1 t2 => GTCase a (compute_term1_kont_graph_dep t1 G) (compute_term1_kont_graph_dep t2 G)
+  | TRef a => GTRef a G
+  | TGet a => GTGet a G
+  | TSet a1 a2 => GTSet a1 a2 G
+  | TFree a => GTFree a G
+  | TShift t' => GTShift k (compute_term1_kont_graph_dep t' GKNil)
+  | TReset t' => GTReset (compute_term_kont_graph_dep t' GKNil) G
+  end
+with compute_term1_kont_graph_dep (t : term1) (k : kont) (G : kont_graph k) : term1_kont_graph t k :=
+  match t with
+  | T1 b t' => GT1 b (compute_term_kont_graph_dep t' G)
+  end
+with compute_term2_kont_graph_dep (t : term2) (k : kont) (G : kont_graph k) : term2_kont_graph t k :=
+  match t with
+  | T2 b1 b2 t' => GT2 b1 b2 (compute_term_kont_graph_dep t' G)
+  end.
+
+Definition compute_clo1_kont_graph_dep (c : clo1) (k : kont) (G : kont_graph k) : clo1_kont_graph c k :=
+  match c with
+  | C1 env t => GC1 env (compute_term1_kont_graph_dep t G)
+  end.
+
+Record irec_kont : Type := IRecKont { app_irec_kont : term -> kont -> imonad val }.
+
+Fixpoint interpret_term_kont_dep (rec : irec_kont) (t : term) (k : kont) (G : term_kont_graph t k) : imonad val :=
+  match t return term_kont_graph t k -> imonad val with
+  | TAtom a => fun G => interpret_kont_dep rec (GTAtom_inv G) (interpret_atom a)
+  | TFun t' => fun G => interpret_kont_dep rec (GTFun_inv G) (interpret_fun t')
+  | TFix t' => fun G => interpret_kont_dep rec (GTFix_inv G) (interpret_fix t')
+  | TApp a1 a2 => fun G =>
+                    let m1 := interpret_atom a1 in
                     let m2 := interpret_atom a2 in
                     imonad_bind m1
-                      (fun v1 =>
-                         match v1 with
-                         | VFun c => imonad_bind m2 (interpret_clo1_aux go c)
-                         | VFix c => imonad_bind m2 (interpret_clo2_aux go c v1)
-                         (*| VKont k => interpret_kont go_kont k m2*)
-                         | _ => imonad_throw (TypeError "")
-                         end)
-    | TPair a1 a2 => interpret_pair a1 a2
-    | TFst a => interpret_fst a
-    | TSnd a => interpret_snd a
-    | TInl a => interpret_inl a
-    | TInr a => interpret_inr a
-    | TCase a t1 t2 => interpret_case a (interpret_term1_aux go' t1) (interpret_term1_aux go' t2)
-    | TRef a => interpret_ref a
-    | TGet a => interpret_get a
-    | TSet a1 a2 => interpret_set a1 a2
-    | TFree a => interpret_free a
-    | TShift _ => imonad_throw (ControlError "shift without enclosing reset")
-    | TReset t' => interpret_term_kont_aux go_kont t' KNil (fun m => m)
-    end.
+                      (fun v => match v with
+                                | VFun c => interpret_clo1_with (fun t' => app_irec_kont rec t k) c m2
+                                | VFix c => interpret_clo2_with (fun t' => app_irec_kont rec t k) c v m2
+                                | VKont k' => interpret_kont_dep rec (GTApp_inv G) (interpret_kont_with (app_irec_kont rec) k m2)
+                                | _ => imonad_throw (TypeError "")
+                                end)
+  | TLet t1 t2 => fun G => imonad_bind imonad_ask_env (fun env => interpret_term_kont_dep rec (GTLet_inv G env))
+  | TIf a t1 t2 => fun G => interpret_if a (interpret_term_kont_dep rec (GTIf_inv1 G)) (interpret_term_kont_dep rec (GTIf_inv2 G))
+  | TPrim1 p a => fun G => interpret_kont_dep rec (GTPrim1_inv G) (interpret_prim1 p a)
+  | TPrim2 p a1 a2 => fun G => interpret_kont_dep rec (GTPrim2_inv G) (interpret_prim2 p a1 a2)
+  | TPair a1 a2 => fun G => interpret_kont_dep rec (GTPair_inv G) (interpret_pair a1 a2)
+  | TSplit a t' => fun G => interpret_split a (interpret_term2_kont_dep rec (GTSplit_inv G))
+  | TInl a => fun G => interpret_kont_dep rec (GTInl_inv G) (interpret_inl a)
+  | TInr a => fun G => interpret_kont_dep rec (GTInr_inv G) (interpret_inr a)
+  | TCase a t1 t2 => fun G => interpret_case a (interpret_term1_kont_dep rec (GTCase_inv1 G)) (interpret_term1_kont_dep rec (GTCase_inv2 G))
+  | TRef a => fun G => interpret_kont_dep rec (GTRef_inv G) (interpret_ref a)
+  | TGet a => fun G => interpret_kont_dep rec (GTGet_inv G) (interpret_get a)
+  | TSet a1 a2 => fun G => interpret_kont_dep rec (GTSet_inv G) (interpret_set a1 a2)
+  | TFree a => fun G => interpret_kont_dep rec (GTFree_inv G) (interpret_free a)
+  | TShift t' => fun G => interpret_term1_kont_dep rec (GTShift_inv G) (VKont k)
+  | TReset t' => fun G => interpret_kont_dep rec (GTReset_inv2 G) (interpret_term_kont_dep rec (GTReset_inv1 G))
+  end G
+with interpret_term1_kont_dep (rec : irec_kont) (t : term1) (k : kont) (G : term1_kont_graph t k) (v : val) : imonad val :=
+  match t return term1_kont_graph t k -> imonad val with
+  | T1 b t' => fun G => with_binder b v (interpret_term_kont_dep rec (GT1_inv G))
+  end G
+with interpret_term2_kont_dep (rec : irec_kont) (t : term2) (k : kont) (G : term2_kont_graph t k) (v1 v2 : val) : imonad val :=
+  match t return term2_kont_graph t k -> imonad val with
+  | T2 b1 b2 t' => fun G => with_binder b1 v1 (with_binder b2 v2 (interpret_term_kont_dep rec (GT2_inv G)))
+  end G
+with interpret_clo1_kont_dep (rec : irec_kont) (c : clo1) (k : kont) (G : clo1_kont_graph c k) (v : val) : imonad val :=
+  match c return clo1_kont_graph c k -> imonad val with
+  | C1 env t => fun G => with_env env (interpret_term1_kont_dep rec (GC1_inv G) v)
+  end G
+with interpret_kont_dep (rec : irec_kont) (k : kont) (G : kont_graph k) (m : imonad val) : imonad val :=
+  match k return kont_graph k -> imonad val with
+  | KNil => fun _ => m
+  | KCons c k' => fun G => imonad_bind m (interpret_clo1_kont_dep rec (GKCons_inv G))
+  end G.
+
+Unset Implicit Arguments.
+
+Fixpoint compute_kont_graph (k : kont) : kont_graph k :=
+  match k with
+  | KNil => GKNil
+  | KCons c k' => GKCons (compute_clo1_kont_graph_dep c (compute_kont_graph k'))
+  end.
+
+Definition compute_term_kont_graph (t : term) (k : kont) : term_kont_graph t k :=
+  compute_term_kont_graph_dep t (compute_kont_graph k).
+
+Definition interpret_term_kont_aux (rec : irec_kont) (t : term) (k : kont) : imonad val :=
+  interpret_term_kont_dep rec (compute_term_kont_graph t k).
+
+Fixpoint interpret_term_kont (fuel : nat) (t : term) (k : kont) : imonad val :=
+  match fuel with
+  | O => imonad_throw OutOfFuel
+  | S fuel' => interpret_term_kont_aux (IRecKont (interpret_term_kont fuel')) t k
+  end.
+
+Record irec : Type := IRec { app_irec : term -> imonad val; app_kont_irec : term -> kont -> imonad val }.
+
+Fixpoint interpret_term_aux (rec : irec) (t : term) : imonad val :=
+  match t with
+  | TAtom a => interpret_atom a
+  | TFun t' => interpret_fun t'
+  | TFix t' => interpret_fix t'
+  | TApp a1 a2 => let m1 := interpret_atom a1 in
+                  let m2 := interpret_atom a2 in
+                  imonad_bind m1
+                    (fun v => match v with
+                              | VFun c => interpret_clo1_with (app_irec rec) c m2
+                              | VFix c => interpret_clo2_with (app_irec rec) c v m2
+                              | VKont k => interpret_kont_with (app_kont_irec rec) k m2
+                              | _ => imonad_throw (TypeError "not a fun/fix/kont")
+                              end)
+  | TLet t1 t2 => imonad_bind (interpret_term_aux rec t1) (interpret_term1_aux rec t2)
+  | TIf a t1 t2 => interpret_if a (interpret_term_aux rec t1) (interpret_term_aux rec t2)
+  | TPrim1 p a => interpret_prim1 p a
+  | TPrim2 p a1 a2 => interpret_prim2 p a1 a2
+  | TPair a1 a2 => interpret_pair a1 a2
+  | TSplit a t' => interpret_split a (interpret_term2_aux rec t')
+  | TInl a => interpret_inl a
+  | TInr a => interpret_inr a
+  | TCase a t1 t2 => interpret_case a (interpret_term1_aux rec t1) (interpret_term1_aux rec t2)
+  | TRef a => interpret_ref a
+  | TGet a => interpret_get a
+  | TSet a1 a2 => interpret_set a1 a2
+  | TFree a => interpret_free a
+  | TShift _ => imonad_throw (ControlError "shift without enclosing reset")
+  | TReset t' => interpret_term_kont_aux (IRecKont (app_kont_irec rec)) t' KNil
+  end
+with interpret_term1_aux (rec : irec) (t : term1) (v : val) : imonad val :=
+  let (b, t') := t in with_binder b v (interpret_term_aux rec t')
+with interpret_term2_aux (rec : irec) (t : term2) (v1 v2 : val) : imonad val :=
+  let (b1, b2, t') := t in with_binder b1 v1 (with_binder b2 v2 (interpret_term_aux rec t')).
 
 Fixpoint interpret_term (fuel : nat) (t : term) : imonad val :=
   match fuel with
   | O => imonad_throw OutOfFuel
-  | S fuel' => interpret_term_aux (interpret_term fuel') (interpret_term_kont fuel') t
+  | S fuel' => interpret_term_aux (IRec (interpret_term fuel') (interpret_term_kont fuel')) t
   end.
 
-Definition run (fuel : nat) (e : term) : (ierror + val) * istate :=
-  interpret_term fuel e ENil istate_empty.
+Definition run_term (fuel : nat) (t : term) : (ierror + val) * iheap :=
+  imonad_run (interpret_term fuel t) ENil iheap_empty.
 
-Definition eval (fuel : nat) (e : term) : ierror + val :=
-  fst (run fuel e).
+Definition eval_term (fuel : nat) (t : term) : ierror + val :=
+  fst (run_term fuel t).
 
-Definition exec (fuel : nat) (e : term) : istate :=
-  snd (run fuel e).
-
-Import Coerce.
-Local Open Scope Z_scope.
-Example f := TReset (TLet
-                       (TPrim2 P2Mul 6 9)
-                       (T1 (Var "x")
-                          (TLet
-                             (TShift (T1 (Var "k") (Var "k")))
-                             (T1 (Var "y") (TPrim2 P2Add (Var "x") (Var "y")))))).
-Example fx := TLet f (T1 (Var "f") (TApp (Var "f") 10)).
-Compute (eval 2 fx).
-
-Example append_aux :=
-  TFix
-    (T2 (Var "f")
-       (T1 (Var "xs")
-          (TCase (Var "xs")
-             (T1 BAnon (TShift (T1 (Var "k") (Var "k"))))
-             (T1 (Var "p")
-                (TLet
-                   (TFst (Var "p"))
-                   (T1 (Var "x")
-                      (TLet
-                         (TSnd (Var "p"))
-                         (T1 (Var "xs'")
-                            (TLet
-                               (TApp (Var "f") (Var "xs'"))
-                               (T1 (Var "r")
-                                  (TLet
-                                     (TPair (Var "x") (Var "r"))
-                                     (T1 (Var "r'") (TInr (Var "r'")))))))))))))).
-
-Fixpoint encode (xs : list Z) : term :=
-  match xs with
-  | nil => TInl AUnit
-  | cons x xs' => TLet (encode xs') (T1 (Var "xs'") (TLet (TPair x (Var "xs'")) (T1 (Var "xs") (TInr (Var "xs")))))
-  end.
-
-Import List.
-Import ListNotations.
-
-Example append1 xs :=
-  TLet xs (T1 (Var "xs") (TReset (TLet append_aux (T1 (Var "append_aux") (TApp (Var "append_aux") (Var "xs")))))).
-
-Example append2 xs ys :=
-  TLet ys (T1 (Var "ys") (TLet (append1 xs) (T1 (Var "append1") (TApp (Var "append1") (Var "ys"))))).
-
-Example ex1_aux := append1 (encode nil).
-Example ex1 := append2 (encode nil) (encode (1 :: nil)).
-Example ex2 := append2 (encode (List.map (fun n => Z.of_nat n) (ListDef.seq 0 1000))) (encode nil).
-
-Example append_direct :=
-  TFix
-    (T2 (Var "f")
-       (T1 (Var "xs")
-          (TFun
-             (T1 (Var "ys")
-                (TCase (Var "xs")
-                   (T1 BAnon (Var "ys"))
-                   (T1 (Var "p")
-                      (TLet
-                         (TFst (Var "p"))
-                         (T1 (Var "x")
-                            (TLet
-                               (TSnd (Var "p"))
-                               (T1 (Var "xs'")
-                                  (TLet
-                                     (TApp (Var "f") (Var "xs'"))
-                                     (T1 (Var "f")
-                                        (TLet
-                                           (TApp (Var "f") (Var "ys"))
-                                           (T1 (Var "r")
-                                              (TLet
-                                                 (TPair (Var "x") (Var "r"))
-                                                 (T1 (Var "r'") (TInr (Var "r'")))))))))))))))))).
-
-Example append xs ys :=
-  TLet xs
-    (T1 (Var "xs")
-       (TLet ys
-          (T1 (Var "ys")
-             (TLet append_direct
-                (T1 (Var "append_aux")
-                   (TLet (TApp (Var "append_aux") (Var "xs"))
-                      (T1 (Var "f") (TApp (Var "f") (Var "ys"))))))))).
-
-Definition xs := encode (List.map (fun n => Z.of_nat n) (ListDef.seq 0 1500)).
-
-Example ex3 := append xs (encode nil).
-
-Compute (eval 10 ex1_aux).
-Time Compute (eval 10 ex1).
-Time Compute (interpret_term_kont 2000 xs KNil (fun m => m) ENil istate_empty).
-Time Compute (interpret_term 2000 xs ENil istate_empty).
+Definition exec_term (fuel : nat) (t : term) : iheap :=
+  snd (run_term fuel t).
