shift-reset/interpreter/iheap.v
@@ -1,0 +1,23 @@
+From Stdlib Require Import NArith.
+From shift_reset.lib Require option.
+From shift_reset.core Require Import heap syntax loc.
+
+Local Open Scope N_scope.
+
+Record iheap : Type := IHeap { iheap_car : heap; iheap_next_loc : loc }.
+
+Definition iheap_empty : iheap :=
+  IHeap heap_empty (Loc 0).
+
+Definition iheap_ref (v : val) (h : iheap) : option (loc * iheap) :=
+  let l := iheap_next_loc h in
+  option.map (fun h' => (l, IHeap h' (loc_succ l))) (heap_ref l v (iheap_car h)).
+
+Definition iheap_get (l : loc) (h : iheap) : option val :=
+  heap_get l (iheap_car h).
+
+Definition iheap_set (l : loc) (v : val) (h : iheap) : option iheap :=
+  option.map (fun h' => IHeap h' (iheap_next_loc h)) (heap_set l v (iheap_car h)).
+
+Definition iheap_free (l : loc) (h : iheap) : option iheap :=
+  option.map (fun h' => IHeap h' (iheap_next_loc h)) (heap_free l (iheap_car h)).
