shift-reset/interpreter/imonad.v
@@ -1,63 +1,72 @@
 From shift_reset.lib Require Import sum.
 From shift_reset.core Require Import syntax.
-From shift_reset.interpreter Require Import istate ierror.
+From shift_reset.interpreter Require Import ierror iheap.
 
-Definition imonad (A : Type) : Type := env -> istate -> (ierror + A) * istate.
+Record imonad (A : Type) : Type := IMonad { imonad_run : env -> iheap -> (ierror + A) * iheap }.
+
+Arguments IMonad {A} _.
+Arguments imonad_run {A} _ _ _.
 
 Definition imonad_ask_env : imonad env :=
-  fun env s => (inr env, s).
+  IMonad (fun env h => (inr env, h)).
 
 Definition imonad_local_env {A} (f : env -> env) (m : imonad A) : imonad A :=
-  fun env s => m (f env) s.
+  IMonad (fun env => imonad_run m (f env)).
 
-Definition imonad_get_state : imonad istate :=
-  fun _ s => (inr s, s).
+Definition imonad_get_heap : imonad iheap :=
+  IMonad (fun _ h => (inr h, h)).
 
-Definition imonad_set_state (s : istate) : imonad unit :=
-  fun _ _ => (inr tt, s).
+Definition imonad_set_heap (h : iheap) : imonad unit :=
+  IMonad (fun _ _ => (inr tt, h)).
 
-Definition imonad_modify_state (f : istate -> istate) : imonad unit :=
-  fun _ s => (inr tt, f s).
+Definition imonad_modify_heap (f : iheap -> iheap) : imonad unit :=
+  IMonad (fun _ h => (inr tt, f h)).
 
 Definition imonad_throw {A} (e : ierror) : imonad A :=
-  fun _ s => (inl e, s).
+  IMonad (fun _ h => (inl e, h)).
 
 Definition imonad_map {A B} (f : A -> B) (m : imonad A) :=
-  fun env s =>
-    let (r, s) := m env s in
-    match r with
-    | inl e => (inl e, s)
-    | inr x => (inr (f x), s)
-    end.
+  IMonad (fun env h =>
+            let (r, h) := imonad_run m env h in
+            match r with
+            | inl e => (inl e, h)
+            | inr x => (inr (f x), h)
+            end).
 
 Definition imonad_pure {A} (x : A) : imonad A :=
-  fun _ s => (inr x, s).
+  IMonad (fun _ h => (inr x, h)).
 
 Definition imonad_lift2 {A B C} (f : A -> B -> C) (m1 : imonad A) (m2 : imonad B) : imonad C :=
-  fun env s =>
-    let (r, s) := m1 env s in
-    match r with
-    | inl e => (inl e, s)
-    | inr x =>
-        let (r, s) := m2 env s in
-        match r with
-        | inl e => (inl e, s)
-        | inr y => (inr (f x y), s)
-        end
-    end.
+  IMonad (fun env h =>
+            let (r, h) := imonad_run m1 env h in
+            match r with
+            | inl e => (inl e, h)
+            | inr x =>
+                let (r, h) := imonad_run m2 env h in
+                match r with
+                | inl e => (inl e, h)
+                | inr y => (inr (f x y), h)
+                end
+            end).
 
 Definition imonad_bind {A B} (m : imonad A) (f : A -> imonad B) : imonad B :=
-  fun env s =>
-    let (r, s) := m env s in
-    match r with
-    | inl e => (inl e, s)
-    | inr x => f x env s
-    end.
+  IMonad (fun env h =>
+            let (r, h) := imonad_run m env h in
+            match r with
+            | inl e => (inl e, h)
+            | inr x => imonad_run (f x) env h
+            end).
 
 Definition imonad_then {A B} (m1 : imonad A) (m2 : imonad B) : imonad B :=
-  fun env s =>
-    let (r, s) := m1 env s in
-    match r with
-    | inl e => (inl e, s)
-    | inr _ => m2 env s
-    end.
+  IMonad (fun env h =>
+            let (r, h) := imonad_run m1 env h in
+            match r with
+            | inl e => (inl e, h)
+            | inr _ => imonad_run m2 env h
+            end).
+
+Definition imonad_eval {A} (m : imonad A) (env : env) (h : iheap) : ierror + A :=
+  fst (imonad_run m env h).
+
+Definition imonad_exec {A} (m : imonad A) (env : env) (h : iheap) : iheap :=
+  snd (imonad_run m env h).
